fixed errors

AVLnode.dfy
@@ -1,7 +1,7 @@
 class AVLnode
 {
-    var node_set: set<AVLnode> 
-    var key_set: set<int>
+    ghost var nodes: set<AVLnode> 
+    ghost var keys: set<int>
 
     var key: int
     var left: AVLnode?
@@ -9,24 +9,44 @@ class AVLnode
     var height: int
 
     constructor (k: int) 
-        ensures node_set == {this}
-        ensures key_set == {k}
+        ensures nodes == {this}
+        ensures keys == {k}
         ensures key == key
         ensures left == null
         ensures right == null
         ensures height == 0
+        ensures valid()
+        ensures balanced()
     {
-        node_set := {this};
-        key_set := {k};
+        nodes := {this};
+        keys := {k};
         key := k;
         left := null;
         right := null;
         height := 0;
     }
 
-    predicate balanced() 
-        reads this, this.left, this.right
+    // need for balance()
+    predicate valid()
+        reads this, nodes
     {
+        this in nodes &&
+        (left != null ==> left in nodes &&
+                        this !in left.nodes &&
+                        left.nodes < nodes && 
+                        forall i :: i in left.keys ==> i < key &&
+                        left.valid()) &&
+        (right != null ==> right in nodes &&
+                        this !in right.nodes &&
+                        right.nodes < nodes && 
+                        forall i :: i in right.keys ==> i > key &&
+                        right.valid()) 
+    }
+
+    predicate balanced() 
+        reads this, nodes
+    {
+        valid() &&
         (left == null && right != null) ==> right.height == 0 &&
         (left != null && right == null) ==> left.height == 0  &&
         (left != null && right != null && left.height >= right.height) ==> left.height - right.height <= 1 &&
