Test.dfy
@@ -3,6 +3,11 @@ include "AVLtree.dfy"
 
 method Test() {
     var avlTree: AVLtree := new AVLtree();
-    var avlNode: AVLnode := new AVLnode(3);
+    var avlNode: AVLnode := new AVLnode(5);
+    assert(avlTree.balanced());
     assert(avlNode.balanced());
+    var height: int := avlTree.nodeHeight(avlTree.root);
+    var heightDiff: int := avlTree.heightDiff(avlTree.root);
+    print(height);
+    print(heightDiff);
 }
